RunBenchmarks.lean
@@ -2,14 +2,16 @@ import MergeSort.Benchmark
 import MergeSort.ArrayGenerators
 
 def main (args :  List String) : IO Unit := do
-  let size := 10 ^ 8
+  let size := 5 * 10 ^ 7
   let seed := 0
-  match args with
-  | ["mergeSort"] =>
-    runOnAllArrayGenerators "Array.mergeSort" size seed Benchmark.Array.mergeSort
-  | ["mergeSortA"] =>
-    runOnAllArrayGenerators "Array.mergeSortA" size seed Benchmark.Array.mergeSortA
-  | _ => panic! "wrong arguments"
+  -- match args with
+  -- | ["mergeSort"] =>
+  --   runOnAllArrayGenerators "Array.mergeSort" size seed Benchmark.Array.mergeSort
+  -- | ["mergeSortA"] =>
+  --   runOnAllArrayGenerators "Array.mergeSortA" size seed Benchmark.Array.mergeSortA
+  -- | _ => panic! "wrong arguments"
+  runOnAllArrayGenerators "safe merge sort" size seed Benchmark.Array.mergeSort
+  runOnAllArrayGenerators "unsafe merge sort" size seed Benchmark.Array.mergeSortA
   -- runOnAllArrayGenerators "List.mergeSort" size seed Benchmark.List.mergeSort
   -- runOnAllArrayGenerators "Array.qsortOrd" size seed Benchmark.Array.qsortOrd
 
